Before: add pure fact to cast

Phi_System/IDE_CP_Reasoning1.thy
@@ -238,12 +238,44 @@ definition \<open>Remove_Values (Input::assn) (Output::assn) \<longleftrightarro
 text \<open>The process \<^prop>\<open>Remove_Values Input Output\<close> removes value assertions \<open>x \<Ztypecolon> \<^bold>v\<^bold>a\<^bold>l T\<close>
   from the assertion \<open>Input\<close>. Bounded values such the return value of a procedure are not removed.\<close>
 
+
 subsection \<open>Collects all Values in an Assertion / from the State Sequent\<close>
 
-lemma Val_inhabited_collect:
-  \<open> Inhabited (x \<Ztypecolon> \<^bold>v\<^bold>a\<^bold>l[v] T) \<Longrightarrow> (sem_value.dest v \<in> (x \<Ztypecolon> T) \<Longrightarrow> C) \<Longrightarrow> C \<close>
-  unfolding Inhabited_def by (clarsimp simp add: \<phi>expns)
+consts collect_clean_value :: \<open>bool \<Rightarrow> unit action\<close>
 
+lemma apply_collect_clean_value:
+  \<open> S \<^bold>i\<^bold>m\<^bold>p\<^bold>l\<^bold>i\<^bold>e\<^bold>s S' \<^bold>a\<^bold>n\<^bold>d V \<^bold><\<^bold>a\<^bold>c\<^bold>t\<^bold>i\<^bold>o\<^bold>n\<^bold>> collect_clean_value WHETHER_CLEAN
+\<Longrightarrow> S \<^bold>i\<^bold>m\<^bold>p\<^bold>l\<^bold>i\<^bold>e\<^bold>s S' \<^bold>a\<^bold>n\<^bold>d V\<close>
+  unfolding Action_Tag_def .
 
+lemma [\<phi>reason 1200 for \<open>?S \<heavy_comma> ?x \<Ztypecolon> \<^bold>v\<^bold>a\<^bold>l[?v] ?T \<^bold>i\<^bold>m\<^bold>p\<^bold>l\<^bold>i\<^bold>e\<^bold>s ?S' \<^bold>a\<^bold>n\<^bold>d ?V \<^bold><\<^bold>a\<^bold>c\<^bold>t\<^bold>i\<^bold>o\<^bold>n\<^bold>> collect_clean_value True\<close>]:
+  \<open> S \<^bold>i\<^bold>m\<^bold>p\<^bold>l\<^bold>i\<^bold>e\<^bold>s S' \<^bold>a\<^bold>n\<^bold>d V \<^bold><\<^bold>a\<^bold>c\<^bold>t\<^bold>i\<^bold>o\<^bold>n\<^bold>> collect_clean_value True
+\<Longrightarrow> S \<heavy_comma> x \<Ztypecolon> \<^bold>v\<^bold>a\<^bold>l[v] T \<^bold>i\<^bold>m\<^bold>p\<^bold>l\<^bold>i\<^bold>e\<^bold>s S' \<^bold>a\<^bold>n\<^bold>d sem_value.dest v \<in> (x \<Ztypecolon> T) \<and> V \<^bold><\<^bold>a\<^bold>c\<^bold>t\<^bold>i\<^bold>o\<^bold>n\<^bold>> collect_clean_value True\<close>
+  unfolding Action_Tag_def Imply_def by (clarsimp simp add: \<phi>expns)
+
+lemma [\<phi>reason 1200 for \<open>?S \<heavy_comma> ?x \<Ztypecolon> \<^bold>v\<^bold>a\<^bold>l[?v] ?T \<^bold>i\<^bold>m\<^bold>p\<^bold>l\<^bold>i\<^bold>e\<^bold>s ?S' \<^bold>a\<^bold>n\<^bold>d ?V \<^bold><\<^bold>a\<^bold>c\<^bold>t\<^bold>i\<^bold>o\<^bold>n\<^bold>> collect_clean_value False\<close>]:
+  \<open> S \<^bold>i\<^bold>m\<^bold>p\<^bold>l\<^bold>i\<^bold>e\<^bold>s S' \<^bold>a\<^bold>n\<^bold>d V \<^bold><\<^bold>a\<^bold>c\<^bold>t\<^bold>i\<^bold>o\<^bold>n\<^bold>> collect_clean_value False
+\<Longrightarrow> S \<heavy_comma> x \<Ztypecolon> \<^bold>v\<^bold>a\<^bold>l[v] T \<^bold>i\<^bold>m\<^bold>p\<^bold>l\<^bold>i\<^bold>e\<^bold>s S' \<heavy_comma> x \<Ztypecolon> \<^bold>v\<^bold>a\<^bold>l[v] T \<^bold>a\<^bold>n\<^bold>d sem_value.dest v \<in> (x \<Ztypecolon> T) \<and> V
+    \<^bold><\<^bold>a\<^bold>c\<^bold>t\<^bold>i\<^bold>o\<^bold>n\<^bold>> collect_clean_value False\<close>
+  unfolding Action_Tag_def Imply_def by (clarsimp simp add: \<phi>expns)
+
+lemma [\<phi>reason 1100 for \<open>?S\<heavy_comma> ?X \<^bold>i\<^bold>m\<^bold>p\<^bold>l\<^bold>i\<^bold>e\<^bold>s ?S' \<^bold>a\<^bold>n\<^bold>d ?V \<^bold><\<^bold>a\<^bold>c\<^bold>t\<^bold>i\<^bold>o\<^bold>n\<^bold>> collect_clean_value ?CLEAN\<close>]:
+  \<open> S \<^bold>i\<^bold>m\<^bold>p\<^bold>l\<^bold>i\<^bold>e\<^bold>s S' \<^bold>a\<^bold>n\<^bold>d V \<^bold><\<^bold>a\<^bold>c\<^bold>t\<^bold>i\<^bold>o\<^bold>n\<^bold>> collect_clean_value CLEAN
+\<Longrightarrow> S\<heavy_comma> X \<^bold>i\<^bold>m\<^bold>p\<^bold>l\<^bold>i\<^bold>e\<^bold>s S'\<heavy_comma> X \<^bold>a\<^bold>n\<^bold>d V \<^bold><\<^bold>a\<^bold>c\<^bold>t\<^bold>i\<^bold>o\<^bold>n\<^bold>> collect_clean_value CLEAN\<close>
+  unfolding Action_Tag_def using implies_right_prod .
+
+lemma [\<phi>reason 1050 for \<open>?x \<Ztypecolon> \<^bold>v\<^bold>a\<^bold>l[?v] ?T \<^bold>i\<^bold>m\<^bold>p\<^bold>l\<^bold>i\<^bold>e\<^bold>s ?S' \<^bold>a\<^bold>n\<^bold>d ?V \<^bold><\<^bold>a\<^bold>c\<^bold>t\<^bold>i\<^bold>o\<^bold>n\<^bold>> collect_clean_value True\<close>]:
+  \<open> x \<Ztypecolon> \<^bold>v\<^bold>a\<^bold>l[v] T \<^bold>i\<^bold>m\<^bold>p\<^bold>l\<^bold>i\<^bold>e\<^bold>s Void \<^bold>a\<^bold>n\<^bold>d sem_value.dest v \<in> (x \<Ztypecolon> T) \<and> True
+    \<^bold><\<^bold>a\<^bold>c\<^bold>t\<^bold>i\<^bold>o\<^bold>n\<^bold>> collect_clean_value True\<close>
+  unfolding Action_Tag_def Imply_def by (clarsimp simp add: \<phi>expns)
+
+lemma [\<phi>reason 1050 for \<open>?x \<Ztypecolon> \<^bold>v\<^bold>a\<^bold>l[?v] ?T \<^bold>i\<^bold>m\<^bold>p\<^bold>l\<^bold>i\<^bold>e\<^bold>s ?S' \<^bold>a\<^bold>n\<^bold>d ?V \<^bold><\<^bold>a\<^bold>c\<^bold>t\<^bold>i\<^bold>o\<^bold>n\<^bold>> collect_clean_value False\<close>]:
+  \<open> x \<Ztypecolon> \<^bold>v\<^bold>a\<^bold>l[v] T \<^bold>i\<^bold>m\<^bold>p\<^bold>l\<^bold>i\<^bold>e\<^bold>s Void \<^bold>a\<^bold>n\<^bold>d sem_value.dest v \<in> (x \<Ztypecolon> T) \<and> True
+    \<^bold><\<^bold>a\<^bold>c\<^bold>t\<^bold>i\<^bold>o\<^bold>n\<^bold>> collect_clean_value False\<close>
+  unfolding Action_Tag_def Imply_def by (clarsimp simp add: \<phi>expns)
+
+lemma [\<phi>reason 1000 for \<open>?S \<^bold>i\<^bold>m\<^bold>p\<^bold>l\<^bold>i\<^bold>e\<^bold>s ?S' \<^bold>a\<^bold>n\<^bold>d ?V \<^bold><\<^bold>a\<^bold>c\<^bold>t\<^bold>i\<^bold>o\<^bold>n\<^bold>> collect_clean_value ?clean\<close>]:
+  \<open> X \<^bold>i\<^bold>m\<^bold>p\<^bold>l\<^bold>i\<^bold>e\<^bold>s X \<^bold>a\<^bold>n\<^bold>d True \<^bold><\<^bold>a\<^bold>c\<^bold>t\<^bold>i\<^bold>o\<^bold>n\<^bold>> collect_clean_value clean\<close>
+  unfolding Action_Tag_def using implies_refl .
 
 end
